Add renewal lemma; next step is to fix proof of existing PB RPCs

src/program_proof/simplepb/renewable_lease.v
@@ -21,13 +21,13 @@ Definition own_lease_expiration γl (t:u64) :=
   mono_nat_auth_own γl (1/2) (int.nat t)
 .
 
-Definition isLease N γl (R:iProp Σ) : iProp Σ :=
+Definition is_lease N γl (R:iProp Σ) : iProp Σ :=
   ∃ γtok,
   inv N (∃ expirationTime, own_lease_expiration γl expirationTime ∗
-        (R ∨ is_time_lb expirationTime ∗ (R ∨ ghost_var γtok 1 ())))
+         (R ∨ is_time_lb expirationTime ∗ (R ∨ ghost_var γtok 1 ())))
 .
 
-Definition postLease N γl (R:iProp Σ) : iProp Σ :=
+Definition post_lease N γl (R:iProp Σ) : iProp Σ :=
   ∀ expirationTime,
   own_lease_expiration γl expirationTime -∗
   is_time_lb expirationTime ={↑N}=∗
@@ -37,7 +37,7 @@ Definition postLease N γl (R:iProp Σ) : iProp Σ :=
 Lemma lease_acc N e R γl t :
   int.nat t < int.nat e →
   is_lease_valid_lb γl e -∗
-  isLease N γl R -∗
+  is_lease N γl R -∗
   £ 1 -∗
   own_time t ={↑N,∅}=∗
   R ∗ (R ={∅,↑N}=∗ own_time t)
@@ -66,8 +66,8 @@ Qed.
 Lemma lease_alloc e N R :
   R ={↑N}=∗
   ∃ γl,
-  isLease N γl R ∗
-  postLease N γl R ∗
+  is_lease N γl R ∗
+  post_lease N γl R ∗
   own_lease_expiration γl e
 .
 Proof.
@@ -107,5 +107,41 @@ Proof.
   }
   { iExists _. iFrame. }
 Qed.
+
+Lemma renew_lease e' γl e t N R :
+  int.nat t < int.nat e →
+  int.nat e < int.nat e' →
+  is_lease N γl R -∗
+  own_lease_expiration γl e -∗
+  own_time t ={↑N}=∗
+  own_time t ∗ own_lease_expiration γl e'
+.
+Proof.
+  intros ??.
+  iIntros "#Hlease Hexp Htime".
+  iDestruct "Hlease" as (γtok) "#Hinv".
+  iInv "Hinv" as "Hi" "Hclose".
+  iDestruct "Hi" as (?) "[>Hexp2 Hi]".
+  iDestruct (mono_nat_auth_own_agree with "Hexp Hexp2") as %[_ Hagree].
+  assert (expirationTime = e) by word.
+  subst.
+  iDestruct "Hi" as "[HR|[>Hbad _]]".
+  2: {
+    iDestruct (mono_nat_lb_own_valid with "Htime Hbad") as %[_ Hbad].
+    exfalso. lia.
+  }
+  iCombine "Hexp Hexp2" as "Hexp".
+  iMod (mono_nat_own_update with "Hexp") as "[Hexp _]".
+  { instantiate (1:=int.nat e'). lia. }
+  iDestruct "Hexp" as "[Hexp Hexp2]".
+  iFrame.
+  iMod ("Hclose" with "[-]"); last done.
+  iExists _; iFrame.
+Qed.
+
+Lemma lease_get_lb γl e :
+  own_lease_expiration γl e -∗
+  is_lease_valid_lb γl e.
+Proof. iApply mono_nat_lb_own_get. Qed.
 
 End renewable_lease_protocol.
